aneris/examples/crdt/statelib/proof/stlib_proof_setup.v
@@ -1,0 +1,152 @@
+From stdpp Require Import gmap.
+
+From iris.base_logic Require Import invariants bi.
+From iris.algebra Require Import agree auth excl gmap.
+
+From aneris.algebra Require Import monotone.
+From aneris.aneris_lang
+  Require Import lang network tactics proofmode lifting resources.
+From aneris.aneris_lang.lib
+  Require Import list_proof lock_proof vector_clock_proof serialization_proof
+    map_proof lock_proof network_util_proof inject.
+From aneris.aneris_lang.lib.serialization Require Import serialization_proof.
+From aneris.aneris_lang.lib.vector_clock Require Import vector_clock_proof.
+From aneris.aneris_lang.program_logic Require Import lightweight_atomic.
+From aneris.prelude Require Import misc time.
+
+From aneris.examples.crdt.spec
+  Require Import crdt_events crdt_resources crdt_denot crdt_time crdt_base.
+From aneris.examples.crdt.statelib.resources
+  Require Import resources_update resources utils resources_utils
+    resources_inv resources_local resources_global resources_lock
+    resources_allocation.
+
+From aneris.examples.crdt.statelib Require Import statelib_code.
+From aneris.examples.crdt.statelib.user_model
+  Require Import params model semi_join_lattices.
+From aneris.examples.crdt.statelib.time Require Import time.
+From aneris.examples.crdt.statelib.STS
+  Require Import utils gst lst mutation merge.
+From aneris.examples.crdt.statelib.proof
+  Require Import spec events utils
+    stlib_proof_utils internal_specs stlib_proof.
+
+Instance timeinst : Log_Time := timestamp_time.
+
+
+
+Section StLibSetup.
+
+  Context `{LogOp: Type, LogSt : Type,
+            !anerisG Mdl Σ, !EqDecision LogOp, !Countable LogOp,
+            !CRDT_Params, !Lattice LogSt, !StLib_Params LogOp LogSt,
+            !Internal_StLibG LogOp Σ}.
+
+  Notation princ_ev := (@principal (gset (Event LogOp)) cc_subseteq).
+
+  (* TODO: cleanup *)
+  Ltac rewrite_lookup := repeat (
+    match goal with
+    | [ H1 : _ !! ?i = Some ?v1, H2 : _ !! ?i = Some ?v2 |- _ ] =>
+          rewrite H1 in H2; inversion H2
+    end); subst.
+
+  (* The following lemma is inspired by the OpLib corresponding lemma *)
+  Lemma stlib_setup E :
+    True ⊢ |={E}=> ∃ (GNames : StLib_GhostNames),
+      StLib_GlobalInv ∗
+      StLib_OwnGlobalState ∅ ∗
+      (∃ (S: gset (fin (length CRDT_Addresses))),
+        (∀ i, ⌜i ∈ S⌝)
+        ∗ [∗ set] f ∈ S, stlib_init_token f) ∗
+      internal_init_spec.
+  Proof.
+    iIntros (_).
+    iMod (alloc_loc_own with "[//]") as (γ_own) "(%S & %HS_def & HS_own0 & HS_own1 & HS_own2)".
+    iMod (alloc_loc_for with "[//]") as (γ_for) "(%S' & %HS'_def & HS_for0 & HS_for1)".
+      assert(S' = S) as ->; [ by apply set_eq | clear HS'_def ].
+    iMod (alloc_loc_sub with "[//]") as (γ_sub) "(%S' & %HS'_def & HS_sub0 & HS_sub1)".
+      assert(S' = S) as ->; [ by apply set_eq | clear HS'_def ].
+    iMod (alloc_loc_cc  with "[//]") as (γ_cc)  "(%S' & %HS'_def & HS_cc_auth & #HS_cc_frag)".
+      assert(S' = S) as ->; [ by apply set_eq | clear HS'_def ].
+    iMod (alloc_loc_cc' with "[//]") as (γ_cc') "(%S' & %HS'_def & HS_cc'_auth & #HS_cc'_frag)".
+      assert(S' = S) as ->; [ by apply set_eq | clear HS'_def ].
+    iMod (alloc_global  with "[//]") as (γ_global) "[Hglobal Hglobal']".
+    iMod (alloc_global_snap  with "[//]") as (γ_global_snap) "[Hglobal_snap_auth #Hglobal_snap_snap]".
+    set HNames := (Build_StLib_GhostNames γ_global γ_global_snap γ_own γ_for γ_sub γ_cc γ_cc').
+    iExists HNames.
+    iMod (inv_alloc CRDT_InvName _ (StLib_GlobalInv_prop)
+      with "[HS_own1 HS_for1 HS_sub1 HS_cc_auth HS_cc'_auth Hglobal' Hglobal_snap_auth]")
+      as "#Hinv".
+    { iNext. iExists (∅, vreplicate (length CRDT_Addresses) ∅).
+      iFrame.
+      iSplit; first (iPureIntro; apply gst_init_valid).
+      iExists S; first iFrame"%".
+      rewrite /StLib_GlibInv_local_part.
+      iDestruct (big_sepS_sep_2 with "HS_own1 HS_for1") as "HS".
+      iDestruct (big_sepS_sep_2 with "HS_sub1 HS") as "HS".
+      iDestruct (big_sepS_sep_2 with "HS_cc_auth HS") as "HS".
+      iDestruct (big_sepS_sep_2 with "HS_cc'_auth HS") as "HS".
+      iApply (big_sepS_mono with "HS").
+      iIntros (x Hx_in) "(H0 & H1 & H2 & H3 & H4)".
+      repeat iExists ∅. rewrite union_empty_R. iFrame.
+      iPureIntro.
+      by split; first by rewrite vlookup_replicate. }
+    iModIntro.
+    iFrame "Hinv".
+
+    iDestruct (internal_init_spec_holds with "Hinv") as "#Hinit".
+    iFrame "#". iFrame "Hglobal".
+
+    iExists S. iFrame "%".
+    rewrite/stlib_init_token/locstate_tok/lockinv_tok.
+    iDestruct (big_sepS_sep_2 with "HS_own0 HS_for0") as "HS".
+    iDestruct (big_sepS_sep_2 with "HS_own2 HS") as "HS".
+    iDestruct (big_sepS_sep_2 with "HS_sub0 HS") as "HS".
+    iDestruct (big_sepS_sep_2 with "HS_cc_frag HS") as "HS".
+    (*iDestruct (big_sepS_sep_2 with "HS_cc'_frag HS") as "HS".*)
+    iApply (big_sepS_mono with "HS").
+    iIntros (x Hx_in) "(H0 & H1 & H2 & H3 & H4)".
+    iFrame.
+  Qed.
+
+End StLibSetup.
+
+(** TODO: setup the library for aient to use:
+  * From true, derive the existence of initial resources (using the above
+  * section)
+  * + init spec. *)
+
+Section Instantiation.
+
+  Context {LogOp LogSt : Type}.
+  Context `{!anerisG Mdl Σ, !EqDecision LogOp, !Countable LogOp,
+            !CRDT_Params, !Lattice LogSt, !StLib_Params LogOp LogSt,
+            !Internal_StLibG LogOp Σ}.
+
+  Global Instance init_fun_instance : StLib_Init_Function := {
+    init := statelib_init
+      StLib_StSerialization.(s_serializer).(s_ser)
+      StLib_StSerialization.(s_serializer).(s_deser) }.
+
+  Global Instance stlib_res_instance `{!StLib_GhostNames}
+    : StLib_Res LogOp := {
+      StLib_InitToken := stlib_init_token;
+      StLib_SocketProto := socket_proto;
+  }.
+
+  (** TODO: ask Abel whether I should:
+    * - replace this by a proof obligation
+    * - Qed instead of defined
+    *)
+  Global Instance stlib_setup_instance : StLibSetup.
+  Proof.
+    iIntros (E) "_".
+    iMod (stlib_setup with "[//]") as (names) "(#Hinv & Hglob & Htoks & #Hinit)".
+    iModIntro.
+    iExists stlib_res_instance.
+    simpl.
+    iFrame "Hinv Hglob Htoks".
+  Admitted.
+
+End Instantiation.
